first commit

Source/Concurrency/CivlCoreTypes.cs
@@ -309,6 +309,119 @@ namespace Microsoft.Boogie
       });
     }
 
+    /*
+     * HoistAsserts computes the weakest liberal precondition (wlp) of the body
+     * of impl as a collection of AssertCmd's. As a side effect, all AssertCmd's
+     * in any block of impl are removed.
+     *
+     * HoistAsserts assumes that the body of impl does not contain any loops or
+     * calls. The blocks in impl are sorted from entry to exit and processed in
+     * reverse order, thus ensuring that a block is processed only once the wlp
+     * of all its successors has been computed.
+     */
+
+    public static List<AssertCmd> HoistAsserts(Implementation impl, ConcurrencyOptions options)
+    {
+      return HoistAsserts(impl, new List<AssertCmd>(), options);
+    }
+
+    public static List<AssertCmd> HoistAsserts(Implementation impl, List<AssertCmd> postconditions, ConcurrencyOptions options)
+    {
+      Dictionary<Block, List<AssertCmd>> wlps = new Dictionary<Block, List<AssertCmd>>();
+      Graph<Block> dag = Program.GraphFromBlocks(impl.Blocks, false);
+      foreach (var block in dag.TopologicalSort())
+      {
+        if (block.TransferCmd is ReturnCmd)
+        {
+          var wlp = HoistAsserts(block.Cmds, postconditions, options);
+          wlps.Add(block, wlp);
+        }
+        else if (block.TransferCmd is GotoCmd gotoCmd)
+        {
+          var wlp =
+            HoistAsserts(block.Cmds, gotoCmd.LabelTargets.SelectMany(b => wlps[b]).ToList(), options);
+          wlps.Add(block, wlp);
+        }
+        else
+        {
+          throw new Cce.UnreachableException();
+        }
+      }
+      return wlps[impl.Blocks[0]].Select(assertCmd => Forall(impl.LocVars.Union(impl.OutParams), assertCmd)).ToList();
+    }
+
+    private static List<AssertCmd> HoistAsserts(List<Cmd> cmds, List<AssertCmd> postconditions, ConcurrencyOptions options)
+    {
+      for (int i = cmds.Count - 1; i >= 0; i--)
+      {
+        var cmd = cmds[i];
+        if (cmd is AssertCmd assertCmd)
+        {
+          postconditions.Add(assertCmd);
+        } 
+        else if (cmd is AssumeCmd assumeCmd)
+        {
+          QKeyValue Append(QKeyValue assumeAttributes, QKeyValue assertAttributes)
+          {
+            if (assumeAttributes == null)
+            {
+              return assertAttributes;
+            }
+            return new QKeyValue(assumeAttributes.tok, assumeAttributes.Key, assumeAttributes.Params, Append(assumeAttributes.Next, assertAttributes));
+          }
+          postconditions = postconditions
+            .Select(assertCmd => new AssertCmd(assertCmd.tok, Expr.Imp(assumeCmd.Expr, assertCmd.Expr), Append(assumeCmd.Attributes, assertCmd.Attributes)))
+            .ToList();
+        }
+        else if (cmd is AssignCmd assignCmd)
+        {
+          var varToExpr = new Dictionary<Variable, Expr>();
+          var simpleAssignCmd = assignCmd.AsSimpleAssignCmd;
+          for (var j = 0; j < simpleAssignCmd.Lhss.Count; j++)
+          {
+            var lhs = simpleAssignCmd.Lhss[j];
+            var rhs = simpleAssignCmd.Rhss[j];
+            varToExpr.Add(lhs.DeepAssignedVariable, rhs);
+          }
+          postconditions = postconditions.Select(assertCmd =>
+            new AssertCmd(assertCmd.tok, SubstitutionHelper.Apply(varToExpr, assertCmd.Expr), Substitute(assertCmd.Attributes, varToExpr))).ToList();
+        }
+        else if (cmd is HavocCmd havocCmd)
+        {
+          postconditions = postconditions.Select(assertCmd => Forall(havocCmd.Vars.Select(ie => ie.Decl), assertCmd)).ToList();
+        }
+        else if (cmd is UnpackCmd unpackCmd)
+        {
+          var desugaredCmd = (StateCmd) unpackCmd.GetDesugaring(options);
+          postconditions = HoistAsserts(desugaredCmd.Cmds, postconditions, options); // removes precondition assert from desugaredCmd.Cmds
+        }
+        else
+        {
+          throw new Cce.UnreachableException();
+        }
+      }
+      cmds.RemoveAll(cmd => cmd is AssertCmd);
+      return postconditions;
+    }
+
+    private static QKeyValue Substitute(QKeyValue kv, Dictionary<Variable, Expr> always)
+    {
+      if (kv == null)
+      {
+        return null;
+      }
+      var newKv = Substitute(kv.Next, always);
+      if (kv.Key != "add_to_pool")
+      {
+        return new QKeyValue(kv.tok, kv.Key, kv.Params, newKv);
+      }
+      return new QKeyValue(
+        kv.tok,
+        kv.Key,
+        kv.Params.Select(param => param is Expr expr ? SubstitutionHelper.Apply(always, expr) : param).ToList(),
+        newKv);
+    }
+
     private void DropSetChoice(Implementation impl)
     {
       impl.Blocks.ForEach(block =>
@@ -367,87 +480,6 @@ namespace Microsoft.Boogie
         block.Cmds = newCmds;
       });
     }
-
-    /*
-     * HoistAsserts computes the weakest liberal precondition (wlp) of the body
-     * of impl as a collection of AssertCmd's. As a side effect, all AssertCmd's
-     * in any block of impl are removed.
-     *
-     * HoistAsserts assumes that the body of impl does not contain any loops or
-     * calls. The blocks in impl are sorted from entry to exit and processed in
-     * reverse order, thus ensuring that a block is processed only once the wlp
-     * of all its successors has been computed.
-     */
-    private List<AssertCmd> HoistAsserts(Implementation impl, ConcurrencyOptions options)
-    {
-      Dictionary<Block, List<AssertCmd>> wlps = new Dictionary<Block, List<AssertCmd>>();
-      Graph<Block> dag = Program.GraphFromBlocks(impl.Blocks, false);
-      foreach (var block in dag.TopologicalSort())
-      {
-        if (block.TransferCmd is ReturnCmd)
-        {
-          var wlp = HoistAsserts(block.Cmds, new List<AssertCmd>(), options);
-          wlps.Add(block, wlp);
-        }
-        else if (block.TransferCmd is GotoCmd gotoCmd)
-        {
-          var wlp =
-            HoistAsserts(block.Cmds, gotoCmd.LabelTargets.SelectMany(b => wlps[b]).ToList(), options);
-          wlps.Add(block, wlp);
-        }
-        else
-        {
-          throw new Cce.UnreachableException();
-        }
-      }
-      return wlps[impl.Blocks[0]].Select(assertCmd => Forall(impl.LocVars.Union(impl.OutParams), assertCmd)).ToList();
-    }
-
-    private List<AssertCmd> HoistAsserts(List<Cmd> cmds, List<AssertCmd> postconditions, ConcurrencyOptions options)
-    {
-      for (int i = cmds.Count - 1; i >= 0; i--)
-      {
-        var cmd = cmds[i];
-        if (cmd is AssertCmd assertCmd)
-        {
-          postconditions.Add(assertCmd);
-        } 
-        else if (cmd is AssumeCmd assumeCmd)
-        {
-          postconditions = postconditions
-            .Select(assertCmd => new AssertCmd(assertCmd.tok, Expr.Imp(assumeCmd.Expr, assertCmd.Expr))).ToList();
-        }
-        else if (cmd is AssignCmd assignCmd)
-        {
-          var varToExpr = new Dictionary<Variable, Expr>();
-          var simpleAssignCmd = assignCmd.AsSimpleAssignCmd;
-          for (var j = 0; j < simpleAssignCmd.Lhss.Count; j++)
-          {
-            var lhs = simpleAssignCmd.Lhss[j];
-            var rhs = simpleAssignCmd.Rhss[j];
-            varToExpr.Add(lhs.DeepAssignedVariable, rhs);
-          }
-          postconditions = postconditions.Select(assertCmd =>
-            new AssertCmd(assertCmd.tok, SubstitutionHelper.Apply(varToExpr, assertCmd.Expr))).ToList();
-        }
-        else if (cmd is HavocCmd havocCmd)
-        {
-          postconditions = postconditions.Select(assertCmd => Forall(havocCmd.Vars.Select(ie => ie.Decl), assertCmd))
-            .ToList();
-        }
-        else if (cmd is UnpackCmd unpackCmd)
-        {
-          var desugaredCmd = (StateCmd) unpackCmd.GetDesugaring(options);
-          postconditions = HoistAsserts(desugaredCmd.Cmds, postconditions, options); // removes precondition assert from desugaredCmd.Cmds
-        }
-        else
-        {
-          throw new Cce.UnreachableException();
-        }
-      }
-      cmds.RemoveAll(cmd => cmd is AssertCmd);
-      return postconditions;
-    }
     
     private static AssertCmd Forall(IEnumerable<Variable> vars, AssertCmd assertCmd)
     {
@@ -458,10 +490,38 @@ namespace Microsoft.Boogie
       {
         return assertCmd;
       }
+
+      bool KeepExpr(Expr expr)
+      {
+        var freeObjects = new GSet<object>();
+        expr.ComputeFreeVariables(freeObjects);
+        return freeObjects.OfType<Variable>().Intersect(vars).Count() == 0;
+      }
+
+      QKeyValue Filter(QKeyValue kv)
+      {
+        if (kv == null)
+        {
+          return null;
+        }
+        var newKv = Filter(kv.Next);
+        if (kv.Key != "add_to_pool")
+        {
+          return new QKeyValue(kv.tok, kv.Key, kv.Params, newKv);
+        }
+        return new QKeyValue(
+          kv.tok,
+          kv.Key,
+          kv.Params.Where(param => param is not Expr expr || KeepExpr(expr)).ToList(),
+          newKv);
+      }
+
       var varMapping = quantifiedVars.ToDictionary(v => v,
-        v => (Variable) VarHelper.BoundVariable(v.Name, v.TypedIdent.Type));
-      return new AssertCmd(assertCmd.tok,
-        ExprHelper.ForallExpr(varMapping.Values.ToList(), SubstitutionHelper.Apply(varMapping, assertCmd.Expr)));
+        v => (Variable) VarHelper.BoundVariable(v.Name, v.TypedIdent.Type, v.Attributes));
+      return new AssertCmd(
+        assertCmd.tok,
+        ExprHelper.ForallExpr(varMapping.Values.ToList(), SubstitutionHelper.Apply(varMapping, assertCmd.Expr)),
+        Filter(assertCmd.Attributes));
     }
     
     private void DeclareTriggerFunctions()
