Source/Concurrency/CivlUtil.cs
@@ -344,9 +344,9 @@ namespace Microsoft.Boogie
       return new LocalVariable(Token.NoToken, new TypedIdent(Token.NoToken, name, type));
     }
 
-    public static BoundVariable BoundVariable(string name, Type type)
+    public static BoundVariable BoundVariable(string name, Type type, QKeyValue kv = null)
     {
-      return new BoundVariable(Token.NoToken, new TypedIdent(Token.NoToken, name, type));
+      return new BoundVariable(Token.NoToken, new TypedIdent(Token.NoToken, name, type), kv);
     }
 
     public static Formal Formal(string name, Type type, bool incoming)
@@ -427,6 +427,14 @@ namespace Microsoft.Boogie
     {
       var subst = FromVariableMap(map);
       return Apply(subst, cmds);
+    }
+  }
+
+  public static class RequiresHelper
+  {
+    public static Requires Requires(Expr expr, QKeyValue kv = null)
+    {
+      return new Requires(Token.NoToken, false, expr, null, kv);
     }
   }
 
