Source/Concurrency/MoverCheck.cs
@@ -201,7 +201,7 @@ namespace Microsoft.Boogie
             .Where(v => LinearTypeChecker.FindLinearKind(v) != LinearKind.LINEAR_OUT), frame).ToList();
       foreach (AssertCmd assertCmd in first.FirstGate.Union(second.SecondGate))
       {
-        requires.Add(new Requires(false, assertCmd.Expr));
+        requires.Add(RequiresHelper.Requires(assertCmd.Expr, assertCmd.Attributes));
       }
       if (moverCheckContext != null)
       {
@@ -278,7 +278,7 @@ namespace Microsoft.Boogie
             .Where(v => LinearTypeChecker.FindLinearKind(v) != LinearKind.LINEAR_OUT), frame).ToList();
       foreach (AssertCmd assertCmd in first.FirstGate.Union(second.SecondGate))
       {
-        requires.Add(new Requires(false, assertCmd.Expr));
+        requires.Add(RequiresHelper.Requires(assertCmd.Expr, assertCmd.Attributes));
       }
       if (moverCheckContext != null)
       {
@@ -298,11 +298,15 @@ namespace Microsoft.Boogie
           .Union(frame));
       foreach (AssertCmd assertCmd in first.FirstGate)
       {
+        var firstTok = first.ActionDecl.tok;
+        var firstLoc = string.Format("{0}({1},{2})", firstTok.filename, firstTok.line, firstTok.col);
+        var secondTok = second.ActionDecl.tok;
+        var secondLoc = string.Format("{0}({1},{2})", secondTok.filename, secondTok.line, secondTok.col);
         cmds.Add(
           CmdHelper.AssertCmd(
             assertCmd.tok,
             Expr.Imp(Expr.And(linearityAssumes), assertCmd.Expr),
-            $"Gate of {first.Name} not preserved by {second.Name}"
+            $"Gate of {first.Name} @ {firstLoc} not preserved by {second.Name} @ {secondLoc}"
           )
         );
       }
@@ -347,15 +351,11 @@ namespace Microsoft.Boogie
       var linearTypeChecker = civlTypeChecker.linearTypeChecker;
       List<Requires> requires = 
         DisjointnessAndWellFormedRequires(
-          first.FirstImpl.InParams.Union(second.SecondImpl.InParams)
-            .Where(v => LinearTypeChecker.FindLinearKind(v) != LinearKind.LINEAR_OUT), frame).ToList();
-      Expr firstNegatedGate = Expr.Not(Expr.And(first.FirstGate.Select(a => a.Expr)));
-      firstNegatedGate.Type = Type.Bool; // necessary?
-      requires.Add(new Requires(false, firstNegatedGate));
-      foreach (AssertCmd assertCmd in second.SecondGate)
-      {
-        requires.Add(new Requires(false, assertCmd.Expr));
-      }
+          first.FirstImpl.InParams.Union(second.SecondImpl.InParams).Where(v => LinearTypeChecker.FindLinearKind(v) != LinearKind.LINEAR_OUT), frame).ToList();
+      var wpreAssertCmds = Action.HoistAsserts(second.SecondImpl, first.FirstGate, Options);
+      requires.AddRange(wpreAssertCmds.Select(assertCmd => RequiresHelper.Requires(assertCmd.Expr, assertCmd.Attributes)));
+      requires.AddRange(second.SecondGate.Select(assertCmd => RequiresHelper.Requires(assertCmd.Expr, assertCmd.Attributes)));
+      
       if (moverCheckContext != null)
       {
         checkerName = $"FailurePreservationChecker_{first.Name}_{second.Name}_{moverCheckContext.layer}";
@@ -364,21 +364,21 @@ namespace Microsoft.Boogie
         });
       }
 
+      var cmds = new List<Cmd>();
       IEnumerable<Expr> linearityAssumes =
-        linearTypeChecker.DisjointnessExprForEachDomain(first.FirstImpl.InParams.Union(second.SecondImpl.OutParams)
-          .Union(frame));
-      AssertCmd gateFailureCheck = CmdHelper.AssertCmd(
-        first.tok,
-        Expr.Imp(Expr.And(linearityAssumes), firstNegatedGate),
-        $"Gate failure of {first.Name} not preserved by {second.Name}");
+        linearTypeChecker.DisjointnessExprForEachDomain(first.FirstImpl.InParams.Union(second.SecondImpl.OutParams).Union(frame));
+      cmds.AddRange(linearityAssumes.Select(expr => new AssumeCmd(Token.NoToken, expr)));
 
       List<Variable> inputs = first.FirstImpl.InParams.Union(second.SecondImpl.InParams).ToList();
       List<Variable> outputs = first.FirstImpl.OutParams.Union(second.SecondImpl.OutParams).ToList();
-      var cmds = new List<Cmd>
-      {
-        ActionCallCmd(second, second.SecondImpl),
-        gateFailureCheck
-      };
+      cmds.AddRange(first.FirstGate.Select(
+        assertCmd => {
+          var firstTok = first.ActionDecl.tok;
+          var firstLoc = string.Format("{0}({1},{2})", firstTok.filename, firstTok.line, firstTok.col);
+          var secondTok = second.ActionDecl.tok;
+          var secondLoc = string.Format("{0}({1},{2})", secondTok.filename, secondTok.line, secondTok.col);
+          return CmdHelper.AssertCmd(assertCmd.tok, assertCmd.Expr, $"Gate failure of {first.Name} @ {firstLoc} not preserved by {second.Name} @ {secondLoc}");
+      }));
 
       AddChecker(checkerName, inputs, outputs, new List<Variable>(), requires, cmds);
     }
