Test/civl/samples/array-insert.bpl
@@ -17,6 +17,7 @@ atomic action {:layer 2} INSERT ({:linear} tid: One Tid, v:int)
 modifies A, count;
 {
   var idx:int; // index at which v is written
+  var old_A: [int]int;
 
   assert count >= 0;
   assert sorted(A, count);
@@ -25,11 +26,12 @@ modifies A, count;
   assume (forall i:int :: 0 <= i && i < idx ==> A[i] < v);
   assume (forall i:int :: idx <= i && i < count ==> A[i] >= v);
 
+  old_A := A;
   havoc A;
 
-  assume (forall i:int :: i < idx ==> A[i] == old(A)[i]);
-  assume (forall i:int :: idx < i && i < count ==> A[i+1] == old(A)[i]);
-  assume (forall i:int :: count < i ==> A[i] == old(A)[i]);
+  assume (forall i:int :: i < idx ==> A[i] == old_A[i]);
+  assume (forall i:int :: idx < i && i < count ==> A[i+1] == old_A[i]);
+  assume (forall i:int :: count < i ==> A[i] == old_A[i]);
   assume A[idx] == v;
 
   count := count + 1;
